src/coq/Handlers/MemoryInterpreters.v
@@ -1,60 +1,166 @@
+From Coq Require Import
+     Morphisms.
+
 From Vellvm.Semantics Require Import
      MemoryParams
+     Memory.ErrSID
      LLVMParams
      LLVMEvents.
 
 From Vellvm.Handlers Require Import
-     MemoryModel.
+     MemoryModel
+     MemPropT.
+
+From Vellvm.Utils Require Import
+     StateMonads.
 
 From ITree Require Import
      ITree
      Basics.Basics
+     Eq.Eq
+     Events.StateFacts
      Events.State.
 
 From ExtLib Require Import
+     Structures.Functor
      Structures.Monads.
+
+(* Needs to be after ITree.Events.State *)
+From Vellvm.Utils Require Import
+     PropT.
+
+Import Basics.Basics.Monads.
+Import MonadNotation.
 
 Set Implicit Arguments.
 Set Contextual Implicit.
 
-Module Type MemoryInterpreter (LP : LLVMParams) (MP : MemoryParams LP) (MM : MemoryModel LP MP).
+Module Type MemorySpecInterpreter (LP : LLVMParams) (MP : MemoryParams LP) (MMSP : MemoryModelSpecPrimitives LP MP) (MM : MemoryModelSpec LP MP MMSP).
   Import MM.
+  Import MMSP.
   Import LP.Events.
 
   Section Interpreters.
-    Variable (E F G : Type -> Type).
-    Context `{FailureE -< F} `{UBE -< F} `{PickConcreteMemoryE -< F} `{OOME -< F}.
+    Variable (E F : Type -> Type).
+    Context `{FailureE -< F} `{UBE -< F} `{OOME -< F}.
     Notation Effin := (E +' IntrinsicE +' MemoryE +' F).
     Notation Effout := (E +' F).
 
-    Definition E_trigger : forall R, E R -> (MemStateT (itree Effout) R) :=
-      fun R e => lift (trigger e).
+    Definition MemStateT M := stateT MemState M.
 
-    Definition F_trigger : forall R, F R -> (MemStateT (itree Effout) R) :=
-      fun R e => lift (trigger e).
+    Definition E_trigger : forall R, E R -> (MemStateT (PropT Effout) R) :=
+      fun R e m => fun t => t ≈ r <- trigger e;; ret (m, r).
+
+    Definition F_trigger : forall R, F R -> (MemStateT (PropT Effout) R) :=
+      fun R e m => fun t => t ≈ r <- trigger e;; ret (m, r).
 
     (* TODO: get rid of this silly hack. *)
-    Definition my_handle_memory :
-      forall T : Type, MemoryE T -> MemStateT (itree Effout) T.
+    Definition my_handle_memory_prop :
+      forall T : Type, MemoryE T -> MemStateT (PropT Effout) T.
     Proof.
-      apply handle_memory.
+      intros T MemE.
+      eapply MemPropT_lift_PropT.
+      eapply handle_memory_prop; auto.
     Defined.
 
-    Definition my_handle_intrinsic :
-      forall T : Type, IntrinsicE T -> MemStateT (itree Effout) T.
+    Definition my_handle_intrinsic_prop :
+      forall T : Type, IntrinsicE T -> MemStateT (PropT Effout) T.
     Proof.
-      apply handle_intrinsic.
+      intros T IntE.
+      eapply MemPropT_lift_PropT.
+      eapply handle_intrinsic_prop; auto.
     Defined.
-      
-    Definition interp_memory_h 
+
+    Definition interp_memory_prop_h : forall T, Effin T -> MemStateT (PropT Effout) T
+      := case_ E_trigger (case_ my_handle_intrinsic_prop (case_ my_handle_memory_prop F_trigger)).
+
+    (* TODO: I find the lack of interp_prop here disturbing... *)
+    Definition memory_k_spec
+               {T R : Type}
+               (e : Effin T)
+               (ta : itree Effout T)
+               (k1 : T -> itree Effin R)
+               (k2 : T -> itree Effout R)
+               (t2 : itree Effout R) : Prop
+      := t2 ≈ (bind ta k2).
+
+    Global Instance memory_k_spec_proper {T R : Type} {RR : R -> R -> Prop} {b a : bool} :
+      Proper
+        (eq ==>
+            eq ==>
+            (fun k1 k2 : T -> itree Effin R =>
+               forall x : T, eqit RR b a (k1 x) (k2 x)) ==> eq ==> eq ==> iff)
+        (memory_k_spec).
+    Proof.
+      unfold Proper, respectful.
+      intros x y ? x0 y0 ? x1 y1 ? x2 y2 ? x3 y3 ?; subst.
+      split; cbn; auto.
+    Qed.
+
+    Definition interp_memory_prop {R} (RR : R -> R -> Prop) :
+      itree Effin R -> MemStateT (PropT Effout) R :=
+      fun (t : itree Effin R) (ms : MemState) (t' : itree Effout (MemState * R)) =>
+        interp_prop (fun T e t => exists ms', @interp_memory_prop_h T e ms (fmap (fun x => (ms', x)) t)) (@memory_k_spec) R RR t (fmap snd t').
+  End Interpreters.
+End MemorySpecInterpreter.
+
+Module Type MemoryExecInterpreter (LP : LLVMParams) (MP : MemoryParams LP) (MMEP : MemoryModelExecPrimitives LP MP) (MM : MemoryModelExec LP MP MMEP).
+  Import MM.
+  Import MMEP.
+  Import MMEP.MMSP.
+  Import LP.
+  Import LP.Events.
+  Import LP.PROV.
+
+  (** Specification of the memory model *)
+  Declare Module SPEC_INTERP : MemorySpecInterpreter LP MP MMSP MemSpec.
+  Import SPEC_INTERP.
+  Import MMSP.
+  Import MMSP.MemByte.
+
+  Section Interpreters.
+    Variable (E F : Type -> Type).
+    Context `{FailureE -< F} `{UBE -< F} `{OOME -< F}.
+    Notation Effin := (E +' IntrinsicE +' MemoryE +' F).
+    Notation Effout := (E +' F).
+
+    Definition E_trigger : E ~> MemStateT (itree Effout) :=
+      fun R e m => r <- trigger e;; ret (m, r).
+
+    Definition F_trigger : F ~> MemStateT (itree Effout) :=
+      fun R e m => r <- trigger e;; ret (m, r).
+
+    (* TODO: get rid of this silly hack. *)
+    Definition my_handle_memory {MemM} `{MemMonad MemState AllocationId MemM} : MemoryE ~> MemStateT (itree Effout) :=
+      fun T e ms => lift_err_ub_oom ret (MemMonad_run (handle_memory T e) ms).
+
+    Definition my_handle_intrinsic {MemM} `{MemMonad MemState AllocationId MemM} : IntrinsicE ~> MemStateT (itree Effout) :=
+      fun T e ms => lift_err_ub_oom ret (MemMonad_run (handle_intrinsic T e) ms).
+
+    Definition interp_memory_h {MemM} `{MemMonad MemState AllocationId MemM} : Effin ~> MemStateT (itree Effout)
       := case_ E_trigger (case_ my_handle_intrinsic (case_ my_handle_memory F_trigger)).
 
-    Definition interp_memory :
+    (* TODO: I find the lack of interp_prop here disturbing... *)
+    Definition interp_memory {MemM} `{MemMonad MemState AllocationId MemM} :
       itree Effin ~> MemStateT (itree Effout) :=
       interp_state interp_memory_h.
-  End Interpreters.
-End MemoryInterpreter.
 
-Module Make (LP : LLVMParams) (MP : MemoryParams LP) (MM : MemoryModel LP MP) : MemoryInterpreter LP MP MM.
-  Include MemoryInterpreter LP MP MM.
-End Make.
+    Lemma interp_memory_correct :
+      forall {MemM} `{MM : MemMonad MemState AllocationId MemM} {T} t ms,
+        interp_memory_prop eq t ms (@interp_memory MemM _ _ _ _ _ _ _ _ _ MM T t ms).
+    Proof.
+      intros MemM H2 H3 H4 H5 H6 H7 H8 H9 H10 MM T t ms.
+      unfold interp_memory_prop.
+      unfold interp_memory.
+      unfold interp_state.
+    Admitted.
+  End Interpreters.
+End MemoryExecInterpreter.
+
+Module MakeMemorySpecInterpreter (LP : LLVMParams) (MP : MemoryParams LP) (MMSP : MemoryModelSpecPrimitives LP MP) (MS : MemoryModelSpec LP MP MMSP) <: MemorySpecInterpreter LP MP MMSP MS.
+  Include MemorySpecInterpreter LP MP MMSP MS.
+End MakeMemorySpecInterpreter.
+
+Module MakeMemoryExecInterpreter (LP : LLVMParams) (MP : MemoryParams LP) (MMEP : MemoryModelExecPrimitives LP MP) (ME : MemoryModelExec LP MP MMEP) <: MemoryExecInterpreter LP MP MMEP ME.
+  Include MemoryExecInterpreter LP MP MMEP ME.
+End MakeMemoryExecInterpreter.
