src/coq/Theory/ExpLemmas.v
@@ -191,9 +191,9 @@ Module ExpLemmas (IS : InterpreterStack) (TOP : LLVMTopLevel IS).
 
     Hint Rewrite @bind_ret_l : rwexp.
     Hint Rewrite @translate_ret : rwexp.
-    Hint Rewrite @interp_cfg3_ret : rwexp.
+    Hint Rewrite @interp_cfg2_ret : rwexp.
     Hint Rewrite @translate_bind : rwexp.
-    Hint Rewrite @interp_cfg3_bind : rwexp.
+    Hint Rewrite @interp_cfg2_bind : rwexp.
     Hint Rewrite @translate_trigger : rwexp.
 
     Ltac simplify_translations :=
@@ -219,16 +219,16 @@ Module ExpLemmas (IS : InterpreterStack) (TOP : LLVMTopLevel IS).
       | |- context [trigger (GlobalRead _)] =>
           match goal with
           | h: Maps.lookup _ _ = Some _ |- _ =>
-              rewrite interp_cfg3_GR; [rewrite ?bind_ret_l | eauto]
+              rewrite interp_cfg2_GR; [rewrite ?bind_ret_l | eauto]
           | h: Maps.lookup _ _ = None |- _ =>
-              rewrite interp_cfg3_GR_fail; [rewrite ?bind_ret_l | eauto]
+              rewrite interp_cfg2_GR_fail; [rewrite ?bind_ret_l | eauto]
           end
       | |- context [trigger (LocalRead _)] =>
           match goal with
           | h: Maps.lookup _ _ = Some _ |- _ =>
-              rewrite interp_cfg3_LR; [rewrite ?bind_ret_l | eauto]
+              rewrite interp_cfg2_LR; [rewrite ?bind_ret_l | eauto]
           | h: Maps.lookup _ _ = None |- _ =>
-              rewrite interp_cfg3_LR_fail; [rewrite ?bind_ret_l | eauto]
+              rewrite interp_cfg2_LR_fail; [rewrite ?bind_ret_l | eauto]
           end
       end.
 
@@ -238,11 +238,11 @@ Module ExpLemmas (IS : InterpreterStack) (TOP : LLVMTopLevel IS).
 
   Section ExpLemmas.
     
-    Lemma denote_exp_GR :forall g l m id v τ,
+    Lemma denote_exp_GR :forall g l id v τ,
         Maps.lookup id g = Some v ->
-        ⟦ EXP_Ident (ID_Global id) at τ ⟧e3 g l m
+        ⟦ EXP_Ident (ID_Global id) at τ ⟧e2 g l
                                          ≈
-                                         Ret (m,(l,(g,dvalue_to_uvalue v))).
+                                         Ret (l,(g,dvalue_to_uvalue v)).
     Proof.
       intros; cbn.
       go.
@@ -251,9 +251,9 @@ Module ExpLemmas (IS : InterpreterStack) (TOP : LLVMTopLevel IS).
       reflexivity.
     Qed.
 
-    Lemma denote_exp_LR :forall g l m id v τ,
+    Lemma denote_exp_LR :forall g l id v τ,
         Maps.lookup id l = Some v ->
-        ⟦ EXP_Ident (ID_Local id) at τ ⟧e3 g l m ≈ Ret (m,(l,(g,v))).
+        ⟦ EXP_Ident (ID_Local id) at τ ⟧e2 g l ≈ Ret (l,(g,v)).
     Proof.
       intros; cbn.
       go.
@@ -262,10 +262,10 @@ Module ExpLemmas (IS : InterpreterStack) (TOP : LLVMTopLevel IS).
       reflexivity.
     Qed.
 
-    Lemma denote_exp_i64 :forall t g l m,
-        ⟦ EXP_Integer (Integers.Int64.intval t) at (DTYPE_I 64) ⟧e3 g l m
+    Lemma denote_exp_i64 :forall t g l,
+        ⟦ EXP_Integer (Integers.Int64.intval t) at (DTYPE_I 64) ⟧e2 g l
                                                                  ≈
-                                                                 Ret (m, (l, (g, UVALUE_I64 t))).
+                                                                 Ret (l, (g, UVALUE_I64 t)).
     Proof.
       intros; cbn.
       go.
@@ -275,10 +275,10 @@ Module ExpLemmas (IS : InterpreterStack) (TOP : LLVMTopLevel IS).
       reflexivity.
     Qed.
 
-    Lemma denote_exp_i64_repr :forall t g l m,
-        ⟦ EXP_Integer t at (DTYPE_I 64) ⟧e3 g l m
+    Lemma denote_exp_i64_repr :forall t g l,
+        ⟦ EXP_Integer t at (DTYPE_I 64) ⟧e2 g l
                                          ≈
-                                         Ret (m, (l, (g, UVALUE_I64 (repr t)))).
+                                         Ret (l, (g, UVALUE_I64 (repr t))).
     Proof.
       intros; cbn.
       go.
@@ -287,10 +287,10 @@ Module ExpLemmas (IS : InterpreterStack) (TOP : LLVMTopLevel IS).
       reflexivity.
     Qed.
 
-    Lemma denote_exp_double :forall t g l m,
-        ⟦ EXP_Double t at DTYPE_Double ⟧e3 g l m
+    Lemma denote_exp_double :forall t g l,
+        ⟦ EXP_Double t at DTYPE_Double ⟧e2 g l
                                         ≈
-                                        Ret (m, (l, (g, UVALUE_Double t))).
+                                        Ret (l, (g, UVALUE_Double t)).
     Proof.
       intros; cbn.
       go.
@@ -429,730 +429,730 @@ Module ExpLemmas (IS : InterpreterStack) (TOP : LLVMTopLevel IS).
      *)
   End ExpLemmas.
 
-  Section ExpPure.
+  (* Section ExpPure. *)
 
-    Import ITreeNotations.
+  (*   Import ITreeNotations. *)
 
-    (* Expressions are "almost pure" computations:
-   they depend on the memory, but do not modify any component on the state *)
+  (*   (* Expressions are "almost pure" computations: *)
+  (*  they depend on the memory, but do not modify any component on the state *) *)
 
-    Definition pure_P g l m : state_cfgP := fun '(m',(l',g')) => m' = m /\ l' = l /\ g' = g.
+  (*   Definition pure_P g l m : state_cfgP := fun '(m',(l',g')) => m' = m /\ l' = l /\ g' = g. *)
 
-    Definition pure {E R} (t : global_env -> local_env -> MemState -> itree E (MemState * (local_env * (global_env * R)))) : Prop :=
-      forall g l m, t g l m ⤳ ↑ (pure_P g l m).
+  (*   Definition pure {E R} (t : global_env -> local_env -> itree E (local_env * (global_env * R))) : Prop := *)
+  (*     forall g l m, t g l m ⤳ ↑ (pure_P g l m). *)
 
-    Lemma failure_is_pure : forall R s,
-        pure (R := R) (interp_cfg3 (raise s)).
-    Proof.
-      unfold pure, raise; intros.
-      go.
-      unfold interp_cfg3.
-      rewrite interp_intrinsics_trigger.
-      cbn.
-      unfold Intrinsics.F_trigger; cbn.
-      rewrite subevent_subevent.
-      rewrite interp_global_trigger; cbn.
-      rewrite subevent_subevent.
-      rewrite interp_local_bind, interp_local_trigger; cbn.
-      rewrite subevent_subevent, bind_bind.
-      rewrite interp_memory_bind, interp_memory_trigger; cbn.
-      rewrite subevent_subevent, !bind_bind.
-      apply has_post_bind; intros [].
-    Qed.
+  (*   Lemma failure_is_pure : forall R s, *)
+  (*       pure (R := R) (interp_cfg3 (raise s)). *)
+  (*   Proof. *)
+  (*     unfold pure, raise; intros. *)
+  (*     go. *)
+  (*     unfold interp_cfg3. *)
+  (*     rewrite interp_intrinsics_trigger. *)
+  (*     cbn. *)
+  (*     unfold Intrinsics.F_trigger; cbn. *)
+  (*     rewrite subevent_subevent. *)
+  (*     rewrite interp_global_trigger; cbn. *)
+  (*     rewrite subevent_subevent. *)
+  (*     rewrite interp_local_bind, interp_local_trigger; cbn. *)
+  (*     rewrite subevent_subevent, bind_bind. *)
+  (*     rewrite interp_memory_bind, interp_memory_trigger; cbn. *)
+  (*     rewrite subevent_subevent, !bind_bind. *)
+  (*     apply has_post_bind; intros []. *)
+  (*   Qed. *)
 
-    Ltac step :=
-      match goal with
-      | |- context [trigger (GlobalRead _)] =>
-          match goal with
-          | h: Maps.lookup _ _ = Some _ |- _ =>
-              rewrite interp_cfg3_GR; [rewrite ?bind_ret_l | eauto]
-          | h: Maps.lookup _ _ = None |- _ =>
-              rewrite interp_cfg3_GR_fail; [rewrite ?bind_ret_l | eauto]
-          end
-      | |- context [trigger (LocalRead _)] =>
-          match goal with
-          | h: Maps.lookup _ _ = Some _ |- _ =>
-              rewrite interp_cfg3_LR; [rewrite ?bind_ret_l | eauto]
-          | h: Maps.lookup _ _ = None |- _ =>
-              rewrite interp_cfg3_LR_fail; [rewrite ?bind_ret_l | eauto]
-          end
-      | |- context [trigger (pick_uvalue _ _)] => rewrite interp_cfg3_pick
-      | |- context [trigger (ThrowUB _)] => rewrite interp_cfg3_UB
-      end.
+  (*   Ltac step := *)
+  (*     match goal with *)
+  (*     | |- context [trigger (GlobalRead _)] => *)
+  (*         match goal with *)
+  (*         | h: Maps.lookup _ _ = Some _ |- _ => *)
+  (*             rewrite interp_cfg3_GR; [rewrite ?bind_ret_l | eauto] *)
+  (*         | h: Maps.lookup _ _ = None |- _ => *)
+  (*             rewrite interp_cfg3_GR_fail; [rewrite ?bind_ret_l | eauto] *)
+  (*         end *)
+  (*     | |- context [trigger (LocalRead _)] => *)
+  (*         match goal with *)
+  (*         | h: Maps.lookup _ _ = Some _ |- _ => *)
+  (*             rewrite interp_cfg3_LR; [rewrite ?bind_ret_l | eauto] *)
+  (*         | h: Maps.lookup _ _ = None |- _ => *)
+  (*             rewrite interp_cfg3_LR_fail; [rewrite ?bind_ret_l | eauto] *)
+  (*         end *)
+  (*     | |- context [trigger (pick_uvalue _ _)] => rewrite interp_cfg3_pick *)
+  (*     | |- context [trigger (ThrowUB _)] => rewrite interp_cfg3_UB *)
+  (*     end. *)
 
-    (* Lemma eval_conv_h_case : forall conv t1 x t2, *)
-    (*         (exists s, eval_conv_h conv t1 x t2 = raise s) \/ *)
-    (*         (exists v, eval_conv_h conv t1 x t2 = Ret v) \/ *)
-    (*         (exists z, eval_conv_h conv t1 x t2 = trigger (ItoP z)) \/ *)
-    (*         (exists z, eval_conv_h conv t1 x t2 = trigger (PtoI t2 z)). *)
-    (* Proof. *)
-    (*   intros. *)
-    (*   unfold eval_conv_h. *)
-    (*   break_match_goal; cbn in *; eauto. *)
-    (* Qed. *)
+  (*   (* Lemma eval_conv_h_case : forall conv t1 x t2, *) *)
+  (*   (*         (exists s, eval_conv_h conv t1 x t2 = raise s) \/ *) *)
+  (*   (*         (exists v, eval_conv_h conv t1 x t2 = Ret v) \/ *) *)
+  (*   (*         (exists z, eval_conv_h conv t1 x t2 = trigger (ItoP z)) \/ *) *)
+  (*   (*         (exists z, eval_conv_h conv t1 x t2 = trigger (PtoI t2 z)). *) *)
+  (*   (* Proof. *) *)
+  (*   (*   intros. *) *)
+  (*   (*   unfold eval_conv_h. *) *)
+  (*   (*   break_match_goal; cbn in *; eauto. *) *)
+  (*   (* Qed. *) *)
 
-    Lemma pick_is_pure : forall u P, pure (ℑ3 (trigger (pick_uvalue P u))).
-    Proof.
-      intros.
-      unfold pure; intros.
-      go.
-      step.
-      apply has_post_bind.
-      intros ?; apply eutt_Ret; cbn; auto.
-    Qed.
+  (*   Lemma pick_is_pure : forall u P, pure (ℑ3 (trigger (pick_uvalue P u))). *)
+  (*   Proof. *)
+  (*     intros. *)
+  (*     unfold pure; intros. *)
+  (*     go. *)
+  (*     step. *)
+  (*     apply has_post_bind. *)
+  (*     intros ?; apply eutt_Ret; cbn; auto. *)
+  (*   Qed. *)
 
-    Lemma UB_is_pure : forall R s,
-        pure (R := R) (ℑ3 (raiseUB s)).
-    Proof.
-      unfold pure, raiseUB; intros.
-      go.
-      step.
-      apply has_post_bind.
-      intros (? & ? & ? & []).
-    Qed.
+  (*   Lemma UB_is_pure : forall R s, *)
+  (*       pure (R := R) (ℑ3 (raiseUB s)). *)
+  (*   Proof. *)
+  (*     unfold pure, raiseUB; intros. *)
+  (*     go. *)
+  (*     step. *)
+  (*     apply has_post_bind. *)
+  (*     intros (? & ? & ? & []). *)
+  (*   Qed. *)
 
-    (* Lemma ItoP_is_pure : forall z, *)
-    (*     pure (ℑ3 (trigger (ItoP z))). *)
-    (* Proof. *)
-    (*   unfold pure; intros. *)
-    (*   unfold ℑ3. *)
-    (*   rewrite interp_intrinsics_trigger. *)
-    (*   cbn. rewrite interp_global_trigger. cbn. *)
-    (*   rewrite interp_local_bind. *)
-    (*   rewrite interp_local_trigger. *)
-    (*   cbn. rewrite bind_trigger. rewrite bind_vis. *)
-    (*   cbn. rewrite interp_memory_vis. cbn. *)
-    (*   break_match; *)
-    (*     try solve [unfold raise; rewrite ?bind_bind; apply has_post_bind; intros []; *)
-    (*   try apply failure_is_pure]. *)
-    (*   1 - 4 : break_match; *)
-    (*     try solve [unfold raise; rewrite ?bind_bind; apply has_post_bind; intros []; *)
-    (*   try apply failure_is_pure]. *)
-    (*   1 - 4 : try destruct p; cbn; setoid_rewrite bind_ret_l; *)
-    (*   rewrite interp_memory_bind; rewrite interp_memory_ret; *)
-    (*   cbn; rewrite bind_ret_l; *)
-    (*   try rewrite interp_local_ret; try rewrite interp_memory_ret; cbn; *)
-    (*     try apply eutt_Ret; cbn; auto. *)
-    (* Qed. *)
+  (*   (* Lemma ItoP_is_pure : forall z, *) *)
+  (*   (*     pure (ℑ3 (trigger (ItoP z))). *) *)
+  (*   (* Proof. *) *)
+  (*   (*   unfold pure; intros. *) *)
+  (*   (*   unfold ℑ3. *) *)
+  (*   (*   rewrite interp_intrinsics_trigger. *) *)
+  (*   (*   cbn. rewrite interp_global_trigger. cbn. *) *)
+  (*   (*   rewrite interp_local_bind. *) *)
+  (*   (*   rewrite interp_local_trigger. *) *)
+  (*   (*   cbn. rewrite bind_trigger. rewrite bind_vis. *) *)
+  (*   (*   cbn. rewrite interp_memory_vis. cbn. *) *)
+  (*   (*   break_match; *) *)
+  (*   (*     try solve [unfold raise; rewrite ?bind_bind; apply has_post_bind; intros []; *) *)
+  (*   (*   try apply failure_is_pure]. *) *)
+  (*   (*   1 - 4 : break_match; *) *)
+  (*   (*     try solve [unfold raise; rewrite ?bind_bind; apply has_post_bind; intros []; *) *)
+  (*   (*   try apply failure_is_pure]. *) *)
+  (*   (*   1 - 4 : try destruct p; cbn; setoid_rewrite bind_ret_l; *) *)
+  (*   (*   rewrite interp_memory_bind; rewrite interp_memory_ret; *) *)
+  (*   (*   cbn; rewrite bind_ret_l; *) *)
+  (*   (*   try rewrite interp_local_ret; try rewrite interp_memory_ret; cbn; *) *)
+  (*   (*     try apply eutt_Ret; cbn; auto. *) *)
+  (*   (* Qed. *) *)
 
-    (* BEGIN TO MOVE *)
-    Lemma FUB_to_exp_raiseUB : forall T s,
-        translate FUB_to_exp (raiseUB (X := T) s) ≈ raiseUB s.
-    Proof.
-      unfold raiseUB; intros.
-      go.
-      apply eutt_eq_bind; intros [].
-    Qed.
+  (*   (* BEGIN TO MOVE *) *)
+  (*   Lemma FUB_to_exp_raiseUB : forall T s, *)
+  (*       translate FUB_to_exp (raiseUB (X := T) s) ≈ raiseUB s. *)
+  (*   Proof. *)
+  (*     unfold raiseUB; intros. *)
+  (*     go. *)
+  (*     apply eutt_eq_bind; intros []. *)
+  (*   Qed. *)
 
-    Lemma exp_to_instr_raiseUB : forall T s,
-        translate exp_to_instr (raiseUB (X := T) s) ≈ raiseUB s.
-    Proof.
-      unfold raiseUB; intros.
-      go.
-      apply eutt_eq_bind; intros [].
-    Qed.
+  (*   Lemma exp_to_instr_raiseUB : forall T s, *)
+  (*       translate exp_to_instr (raiseUB (X := T) s) ≈ raiseUB s. *)
+  (*   Proof. *)
+  (*     unfold raiseUB; intros. *)
+  (*     go. *)
+  (*     apply eutt_eq_bind; intros []. *)
+  (*   Qed. *)
 
-    Lemma FUB_to_exp_raise : forall T s,
-        translate FUB_to_exp (raise (A := T) s) ≈ raise s.
-    Proof.
-      unfold raise; intros.
-      go. 
-      apply eutt_eq_bind; intros [].
-    Qed.
+  (*   Lemma FUB_to_exp_raise : forall T s, *)
+  (*       translate FUB_to_exp (raise (A := T) s) ≈ raise s. *)
+  (*   Proof. *)
+  (*     unfold raise; intros. *)
+  (*     go.  *)
+  (*     apply eutt_eq_bind; intros []. *)
+  (*   Qed. *)
 
-    Lemma exp_to_instr_raise : forall T s,
-        translate exp_to_instr (raise (A := T) s) ≈ raise s.
-    Proof.
-      unfold raise; intros.
-      go. 
-      apply eutt_eq_bind; intros [].
-    Qed.
+  (*   Lemma exp_to_instr_raise : forall T s, *)
+  (*       translate exp_to_instr (raise (A := T) s) ≈ raise s. *)
+  (*   Proof. *)
+  (*     unfold raise; intros. *)
+  (*     go.  *)
+  (*     apply eutt_eq_bind; intros []. *)
+  (*   Qed. *)
 
-    Lemma exp_to_instr_pick : forall P uv,
-        translate exp_to_instr (trigger (pick_uvalue P uv)) ≈ trigger (pick_uvalue P uv).
-    Proof.
-      intros.
-      go. 
-      reflexivity.
-    Qed.
+  (*   Lemma exp_to_instr_pick : forall P uv, *)
+  (*       translate exp_to_instr (trigger (pick_uvalue P uv)) ≈ trigger (pick_uvalue P uv). *)
+  (*   Proof. *)
+  (*     intros. *)
+  (*     go.  *)
+  (*     reflexivity. *)
+  (*   Qed. *)
 
-    Lemma concretize_or_pick_is_pure : forall v P, pure (ℑ3 (translate exp_to_instr (concretize_or_pick v P))).
-    Proof.
-      unfold pure; intros.
-      unfold concretize_or_pick.
-      break_match_goal; [| rewrite exp_to_instr_pick; apply pick_is_pure].
-      unfold lift_err.
-      break_match_goal; [rewrite exp_to_instr_raise; apply failure_is_pure |].
-      cbn.
-      go.
-      apply eutt_Ret; cbn; auto.
-    Qed.
+  (*   Lemma concretize_or_pick_is_pure : forall v P, pure (ℑ3 (translate exp_to_instr (concretize_or_pick v P))). *)
+  (*   Proof. *)
+  (*     unfold pure; intros. *)
+  (*     unfold concretize_or_pick. *)
+  (*     break_match_goal; [| rewrite exp_to_instr_pick; apply pick_is_pure]. *)
+  (*     unfold lift_err. *)
+  (*     break_match_goal; [rewrite exp_to_instr_raise; apply failure_is_pure |]. *)
+  (*     cbn. *)
+  (*     go. *)
+  (*     apply eutt_Ret; cbn; auto. *)
+  (*   Qed. *)
 
-    Lemma translate_map_monad {E F A B} (l : list A) (ts : A -> itree E B) (h : E ~> F) :
-      translate h (map_monad ts l) ≈ map_monad (fun a => translate h (ts a)) l.
-    Proof.
-      induction l as [| a l IH].
-      - cbn; go; reflexivity.
-      - cbn; go. 
-        apply eutt_eq_bind; intros ?.
-        go.
-        rewrite IH.
-        setoid_rewrite translate_ret.
-        reflexivity.
-    Qed.
+  (*   Lemma translate_map_monad {E F A B} (l : list A) (ts : A -> itree E B) (h : E ~> F) : *)
+  (*     translate h (map_monad ts l) ≈ map_monad (fun a => translate h (ts a)) l. *)
+  (*   Proof. *)
+  (*     induction l as [| a l IH]. *)
+  (*     - cbn; go; reflexivity. *)
+  (*     - cbn; go.  *)
+  (*       apply eutt_eq_bind; intros ?. *)
+  (*       go. *)
+  (*       rewrite IH. *)
+  (*       setoid_rewrite translate_ret. *)
+  (*       reflexivity. *)
+  (*   Qed. *)
 
-    Lemma interp_map_monad {E F A B} (l : list A) (ts : A -> itree E B) (h : E ~> itree F):
-      interp h (map_monad ts l) ≈ map_monad (fun a => interp h (ts a)) l.
-    Proof.
-      intros; induction l as [| a l IH]; simpl.
-      - rewrite interp_ret; reflexivity.
-      - rewrite interp_bind.
-        apply eutt_eq_bind; intros ?; cbn.
-        rewrite interp_bind, IH.
-        apply eutt_eq_bind; intros ?; cbn.
-        rewrite interp_ret; reflexivity.
-    Qed.
+  (*   Lemma interp_map_monad {E F A B} (l : list A) (ts : A -> itree E B) (h : E ~> itree F): *)
+  (*     interp h (map_monad ts l) ≈ map_monad (fun a => interp h (ts a)) l. *)
+  (*   Proof. *)
+  (*     intros; induction l as [| a l IH]; simpl. *)
+  (*     - rewrite interp_ret; reflexivity. *)
+  (*     - rewrite interp_bind. *)
+  (*       apply eutt_eq_bind; intros ?; cbn. *)
+  (*       rewrite interp_bind, IH. *)
+  (*       apply eutt_eq_bind; intros ?; cbn. *)
+  (*       rewrite interp_ret; reflexivity. *)
+  (*   Qed. *)
 
-    Lemma interp_state_map_monad {E F S A B} (l : list A) (ts : A -> itree E B) (h : E ~> Monads.stateT S (itree F)) (s : S):
-      interp_state h (map_monad ts l) s ≈ map_monad (m := Monads.stateT S (itree F)) (fun a => interp_state h (ts a)) l s.
-    Proof.
-      intros; revert s; induction l as [| a l IH]; simpl; intros s.
-      - rewrite interp_state_ret; reflexivity.
-      - rewrite interp_state_bind.
-        apply eutt_eq_bind; intros []; cbn.
-        rewrite interp_state_bind, IH.
-        apply eutt_eq_bind; intros []; cbn.
-        rewrite interp_state_ret; reflexivity.
-    Qed.
+  (*   Lemma interp_state_map_monad {E F S A B} (l : list A) (ts : A -> itree E B) (h : E ~> Monads.stateT S (itree F)) (s : S): *)
+  (*     interp_state h (map_monad ts l) s ≈ map_monad (m := Monads.stateT S (itree F)) (fun a => interp_state h (ts a)) l s. *)
+  (*   Proof. *)
+  (*     intros; revert s; induction l as [| a l IH]; simpl; intros s. *)
+  (*     - rewrite interp_state_ret; reflexivity. *)
+  (*     - rewrite interp_state_bind. *)
+  (*       apply eutt_eq_bind; intros []; cbn. *)
+  (*       rewrite interp_state_bind, IH. *)
+  (*       apply eutt_eq_bind; intros []; cbn. *)
+  (*       rewrite interp_state_ret; reflexivity. *)
+  (*   Qed. *)
 
-    (* END TO MOVE *)
+  (*   (* END TO MOVE *) *)
 
-    Lemma interp_cfg3_map_monad {A B} g l m (xs : list A) (ts : A -> itree _ B) : 
-      ℑ3 (map_monad ts xs) g l m ≈
-         map_monad (m := Monads.stateT _ (Monads.stateT _ (Monads.stateT _ (itree _))))
-         (fun a => ℑ3 (ts a)) xs g l m.
-    Proof.
-      intros; revert g l m; induction xs as [| a xs IH]; simpl; intros.
-      - rewrite interp_cfg3_ret; reflexivity.
-      - rewrite interp_cfg3_bind.
-        apply eutt_eq_bind; intros (? & ? & ? & ?); cbn.
-        rewrite interp_cfg3_bind, IH.
-        apply eutt_eq_bind; intros (? & ? & ? & ?); cbn.
-        rewrite interp_cfg3_ret; reflexivity.
-    Qed.
+  (*   Lemma interp_cfg3_map_monad {A B} g l m (xs : list A) (ts : A -> itree _ B) :  *)
+  (*     ℑ3 (map_monad ts xs) g l m ≈ *)
+  (*        map_monad (m := Monads.stateT _ (Monads.stateT _ (Monads.stateT _ (itree _)))) *)
+  (*        (fun a => ℑ3 (ts a)) xs g l m. *)
+  (*   Proof. *)
+  (*     intros; revert g l m; induction xs as [| a xs IH]; simpl; intros. *)
+  (*     - rewrite interp_cfg3_ret; reflexivity. *)
+  (*     - rewrite interp_cfg3_bind. *)
+  (*       apply eutt_eq_bind; intros (? & ? & ? & ?); cbn. *)
+  (*       rewrite interp_cfg3_bind, IH. *)
+  (*       apply eutt_eq_bind; intros (? & ? & ? & ?); cbn. *)
+  (*       rewrite interp_cfg3_ret; reflexivity. *)
+  (*   Qed. *)
 
-    Lemma map_monad_eutt_state_ind :
-      forall {E S A B} (I : S -> Prop) (f : A -> Monads.stateT S (itree E) B) (l : list A) s,
-        (forall a s, In a l -> I s -> (f a s) ⤳ fun '(s,_) => I s) ->
-        I s ->
-        map_monad f l s ⤳ fun '(s,_) => I s.
-    Proof.
-      induction l as [| a l IH]; intros s HB HI; simpl.
-      - apply eutt_Ret; auto.
-      - setoid_rewrite has_post_post_strong in HB.
-        eapply eutt_clo_bind; [apply HB; cbn; auto |].
-        intros [s' ?] [] [EQ ?]; inv EQ.
-        simpl.
-        setoid_rewrite has_post_post_strong in IH.
-        eapply eutt_clo_bind; [apply IH |]; auto.
-        intros; apply HB; cbn; auto. 
-        intros [s' ?] [] [EQ ?]; inv EQ; cbn; apply eutt_Ret; auto. 
-    Qed.
+  (*   Lemma map_monad_eutt_state_ind : *)
+  (*     forall {E S A B} (I : S -> Prop) (f : A -> Monads.stateT S (itree E) B) (l : list A) s, *)
+  (*       (forall a s, In a l -> I s -> (f a s) ⤳ fun '(s,_) => I s) -> *)
+  (*       I s -> *)
+  (*       map_monad f l s ⤳ fun '(s,_) => I s. *)
+  (*   Proof. *)
+  (*     induction l as [| a l IH]; intros s HB HI; simpl. *)
+  (*     - apply eutt_Ret; auto. *)
+  (*     - setoid_rewrite has_post_post_strong in HB. *)
+  (*       eapply eutt_clo_bind; [apply HB; cbn; auto |]. *)
+  (*       intros [s' ?] [] [EQ ?]; inv EQ. *)
+  (*       simpl. *)
+  (*       setoid_rewrite has_post_post_strong in IH. *)
+  (*       eapply eutt_clo_bind; [apply IH |]; auto. *)
+  (*       intros; apply HB; cbn; auto.  *)
+  (*       intros [s' ?] [] [EQ ?]; inv EQ; cbn; apply eutt_Ret; auto.  *)
+  (*   Qed. *)
 
-    Lemma map_monad_eutt_state2_ind :
-      forall {E S1 S2 A B} (I : S1 -> S2 -> Prop)
-             (f : A -> Monads.stateT S1 (Monads.stateT S2 (itree E)) B)
-             (l : list A) (s1 : S1) (s2 : S2), 
-        (forall a s1 s2, In a l -> I s1 s2 -> (f a s1 s2) ⤳ fun '(s2',(s1',_)) => I s1' s2') ->
-        I s1 s2 ->
-        map_monad f l s1 s2 ⤳ fun '(s2',(s1',_)) => I s1' s2'.
-    Proof.
-      induction l as [| a l IH]; intros s1 s2 HB HI; simpl.
-      - apply eutt_Ret; auto.
-      - setoid_rewrite has_post_post_strong in HB.
-        eapply eutt_clo_bind; [apply HB; cbn; auto |].
-        intros (s2' & s1' & ?) (? & ? & ?) [EQ ?]; inv EQ.
-        simpl.
-        setoid_rewrite has_post_post_strong in IH.
-        eapply eutt_clo_bind; [apply IH |]; auto.
-        intros; apply HB; cbn; auto.
-        intros (s1' & s2' & ?) (? & ? & ?) [EQ ?]; inv EQ; cbn; apply eutt_Ret; auto. 
-    Qed.
+  (*   Lemma map_monad_eutt_state2_ind : *)
+  (*     forall {E S1 S2 A B} (I : S1 -> S2 -> Prop) *)
+  (*            (f : A -> Monads.stateT S1 (Monads.stateT S2 (itree E)) B) *)
+  (*            (l : list A) (s1 : S1) (s2 : S2),  *)
+  (*       (forall a s1 s2, In a l -> I s1 s2 -> (f a s1 s2) ⤳ fun '(s2',(s1',_)) => I s1' s2') -> *)
+  (*       I s1 s2 -> *)
+  (*       map_monad f l s1 s2 ⤳ fun '(s2',(s1',_)) => I s1' s2'. *)
+  (*   Proof. *)
+  (*     induction l as [| a l IH]; intros s1 s2 HB HI; simpl. *)
+  (*     - apply eutt_Ret; auto. *)
+  (*     - setoid_rewrite has_post_post_strong in HB. *)
+  (*       eapply eutt_clo_bind; [apply HB; cbn; auto |]. *)
+  (*       intros (s2' & s1' & ?) (? & ? & ?) [EQ ?]; inv EQ. *)
+  (*       simpl. *)
+  (*       setoid_rewrite has_post_post_strong in IH. *)
+  (*       eapply eutt_clo_bind; [apply IH |]; auto. *)
+  (*       intros; apply HB; cbn; auto. *)
+  (*       intros (s1' & s2' & ?) (? & ? & ?) [EQ ?]; inv EQ; cbn; apply eutt_Ret; auto.  *)
+  (*   Qed. *)
 
-    Lemma map_monad_eutt_state3_ind :
-      forall {E S1 S2 S3 A B} (I : S1 -> S2 -> S3 -> Prop)
-             (f : A -> Monads.stateT S1 (Monads.stateT S2 (Monads.stateT S3 (itree E))) B)
-             (l : list A) (s1 : S1) (s2 : S2) (s3 : S3), 
-        (forall a s1 s2 s3, In a l -> I s1 s2 s3 -> (f a s1 s2 s3) ⤳ fun '(s3', (s2',(s1',_))) => I s1' s2' s3') ->
-        I s1 s2 s3 ->
-        map_monad f l s1 s2 s3 ⤳ fun '(s3', (s2',(s1',_))) => I s1' s2' s3'.
-    Proof.
-      induction l as [| a l IH]; intros s1 s2 s3 HB HI; simpl.
-      - apply eutt_Ret; auto.
-      - setoid_rewrite has_post_post_strong in HB.
-        eapply eutt_clo_bind; [apply HB; cbn; auto |].
-        intros (s3' & s2' & s1' & ?) (? & ? & ? & ?) [EQ ?]; inv EQ.
-        simpl.
-        setoid_rewrite has_post_post_strong in IH.
-        eapply eutt_clo_bind; [apply IH |]; auto.
-        intros; apply HB; cbn; auto.
-        intros (s1' & s2' & s3' & ?) (? & ? & ? & ?) [EQ ?]; inv EQ; cbn; apply eutt_Ret; auto. 
-    Qed.
+  (*   Lemma map_monad_eutt_state3_ind : *)
+  (*     forall {E S1 S2 S3 A B} (I : S1 -> S2 -> S3 -> Prop) *)
+  (*            (f : A -> Monads.stateT S1 (Monads.stateT S2 (Monads.stateT S3 (itree E))) B) *)
+  (*            (l : list A) (s1 : S1) (s2 : S2) (s3 : S3),  *)
+  (*       (forall a s1 s2 s3, In a l -> I s1 s2 s3 -> (f a s1 s2 s3) ⤳ fun '(s3', (s2',(s1',_))) => I s1' s2' s3') -> *)
+  (*       I s1 s2 s3 -> *)
+  (*       map_monad f l s1 s2 s3 ⤳ fun '(s3', (s2',(s1',_))) => I s1' s2' s3'. *)
+  (*   Proof. *)
+  (*     induction l as [| a l IH]; intros s1 s2 s3 HB HI; simpl. *)
+  (*     - apply eutt_Ret; auto. *)
+  (*     - setoid_rewrite has_post_post_strong in HB. *)
+  (*       eapply eutt_clo_bind; [apply HB; cbn; auto |]. *)
+  (*       intros (s3' & s2' & s1' & ?) (? & ? & ? & ?) [EQ ?]; inv EQ. *)
+  (*       simpl. *)
+  (*       setoid_rewrite has_post_post_strong in IH. *)
+  (*       eapply eutt_clo_bind; [apply IH |]; auto. *)
+  (*       intros; apply HB; cbn; auto. *)
+  (*       intros (s1' & s2' & s3' & ?) (? & ? & ? & ?) [EQ ?]; inv EQ; cbn; apply eutt_Ret; auto.  *)
+  (*   Qed. *)
 
-    Ltac trivial_cases :=
-      try first [apply eutt_Ret; cbn; auto; fail |
+  (*   Ltac trivial_cases := *)
+  (*     try first [apply eutt_Ret; cbn; auto; fail | *)
 
-                  unfold raise; rewrite ?bind_bind; apply has_post_bind; intros [] |
+  (*                 unfold raise; rewrite ?bind_bind; apply has_post_bind; intros [] | *)
 
-                  match goal with
-                    |- context [raise] => rewrite ?FUB_to_exp_raise, ?exp_to_instr_raise;
-                                          apply failure_is_pure
-                  end |
+  (*                 match goal with *)
+  (*                   |- context [raise] => rewrite ?FUB_to_exp_raise, ?exp_to_instr_raise; *)
+  (*                                         apply failure_is_pure *)
+  (*                 end | *)
 
                   
-                  match goal with
-                    |- context [raiseUB] => rewrite ?FUB_to_exp_raiseUB, ?exp_to_instr_raiseUB; 
-                                            apply UB_is_pure
-                  end |
+  (*                 match goal with *)
+  (*                   |- context [raiseUB] => rewrite ?FUB_to_exp_raiseUB, ?exp_to_instr_raiseUB;  *)
+  (*                                           apply UB_is_pure *)
+  (*                 end | *)
                   
-                  match goal with
-                    |- context [pick_uvalue] => rewrite ?exp_to_instr_pick;
-                                         apply pick_is_pure
-                  end 
+  (*                 match goal with *)
+  (*                   |- context [pick_uvalue] => rewrite ?exp_to_instr_pick; *)
+  (*                                        apply pick_is_pure *)
+  (*                 end  *)
 
-        ].
+  (*       ]. *)
 
-    Ltac intro_pure := intros (? & ? & ? & ?) (-> & -> & ->).
+  (*   Ltac intro_pure := intros (? & ? & ? & ?) (-> & -> & ->). *)
 
-    Lemma conv_to_exp_raise: forall (T : Type) (s : string), translate conv_to_exp (raise (A := T) s) ≈ raise s.
-    Proof.
-      unfold raise; intros.
-      go.
-      apply eutt_eq_bind; intros [].
-    Qed.
+  (*   Lemma conv_to_exp_raise: forall (T : Type) (s : string), translate conv_to_exp (raise (A := T) s) ≈ raise s. *)
+  (*   Proof. *)
+  (*     unfold raise; intros. *)
+  (*     go. *)
+  (*     apply eutt_eq_bind; intros []. *)
+  (*   Qed. *)
 
-    (* Lemma expr_are_pure : forall (o : option dtyp) e, pure ⟦ e at? o ⟧e3. *)
-    (* Proof with trivial_cases. *)
-    (*   intros; unfold pure. *)
-    (*   revert o; induction e; simpl; intros. *)
+  (*   (* Lemma expr_are_pure : forall (o : option dtyp) e, pure ⟦ e at? o ⟧e3. *) *)
+  (*   (* Proof with trivial_cases. *) *)
+  (*   (*   intros; unfold pure. *) *)
+  (*   (*   revert o; induction e; simpl; intros. *) *)
 
-    (*   - destruct id; cbn. *)
-    (*     + go. *)
-    (*       destruct (Maps.lookup id g) eqn:EQ. *)
-    (*       * step. *)
-    (*         go... *)
+  (*   (*   - destruct id; cbn. *) *)
+  (*   (*     + go. *) *)
+  (*   (*       destruct (Maps.lookup id g) eqn:EQ. *) *)
+  (*   (*       * step. *) *)
+  (*   (*         go... *) *)
     
-    (*       * step... *)
+  (*   (*       * step... *) *)
     
-    (*     + go.  *)
-    (*       destruct (Maps.lookup id l) eqn:EQ. *)
-    (*       * step...  *)
-    (*       * step... *)
+  (*   (*     + go.  *) *)
+  (*   (*       destruct (Maps.lookup id l) eqn:EQ. *) *)
+  (*   (*       * step...  *) *)
+  (*   (*       * step... *) *)
     
-    (*   - destruct o; cbn... *)
-    (*     destruct d; simpl... *)
-    (*     unfold denote_exp, lift_undef_or_err. *)
-    (*     cbn. *)
-    (*     break_match_goal...  *)
-    (*     break_match_goal... *)
-    (*     go... *)
+  (*   (*   - destruct o; cbn... *) *)
+  (*   (*     destruct d; simpl... *) *)
+  (*   (*     unfold denote_exp, lift_undef_or_err. *) *)
+  (*   (*     cbn. *) *)
+  (*   (*     break_match_goal...  *) *)
+  (*   (*     break_match_goal... *) *)
+  (*   (*     go... *) *)
 
-    (*   - destruct o; cbn... *)
-    (*     destruct d; simpl... *)
-    (*     go... *)
+  (*   (*   - destruct o; cbn... *) *)
+  (*   (*     destruct d; simpl... *) *)
+  (*   (*     go... *) *)
 
-    (*   - destruct o; cbn... *)
-    (*     destruct d; simpl... *)
-    (*     go... *)
+  (*   (*   - destruct o; cbn... *) *)
+  (*   (*     destruct d; simpl... *) *)
+  (*   (*     go... *) *)
 
-    (*   - destruct o; cbn... *)
-    (*     destruct d; simpl... *)
-    (*     go... *)
-    (*     go... *)
+  (*   (*   - destruct o; cbn... *) *)
+  (*   (*     destruct d; simpl... *) *)
+  (*   (*     go... *) *)
+  (*   (*     go... *) *)
 
-    (*   - destruct b; simpl; go... *)
+  (*   (*   - destruct b; simpl; go... *) *)
 
-    (*   - simpl; go... *)
+  (*   (*   - simpl; go... *) *)
 
-    (*   - destruct o; cbn... *)
+  (*   (*   - destruct o; cbn... *) *)
 
-    (*   - go. *)
-    (*     rewrite translate_map_monad. *)
-    (*     rewrite interp_cfg3_map_monad. *)
-    (*     apply has_post_bind_strong with (S := ↑ (pure_P g l m)). *)
-    (*     + eapply has_post_weaken. *)
-    (*       apply (map_monad_eutt_state3_ind (fun g' l' m' => pure_P g l m (m',(l',g')))); [| cbn; intuition]. *)
-    (*       * intros * IN (-> & -> & ->). *)
-    (*         destruct a; simpl in *. *)
-    (*         apply has_post_weaken with (↑ (pure_P g l m)). *)
-    (*         apply (H _ IN). *)
-    (*         intro_pure; cbn; auto. *)
-    (*       * intro_pure; cbn; auto.  *)
-    (*     + intro_pure. *)
-    (*       go... *)
+  (*   (*   - go. *) *)
+  (*   (*     rewrite translate_map_monad. *) *)
+  (*   (*     rewrite interp_cfg3_map_monad. *) *)
+  (*   (*     apply has_post_bind_strong with (S := ↑ (pure_P g l m)). *) *)
+  (*   (*     + eapply has_post_weaken. *) *)
+  (*   (*       apply (map_monad_eutt_state3_ind (fun g' l' m' => pure_P g l m (m',(l',g')))); [| cbn; intuition]. *) *)
+  (*   (*       * intros * IN (-> & -> & ->). *) *)
+  (*   (*         destruct a; simpl in *. *) *)
+  (*   (*         apply has_post_weaken with (↑ (pure_P g l m)). *) *)
+  (*   (*         apply (H _ IN). *) *)
+  (*   (*         intro_pure; cbn; auto. *) *)
+  (*   (*       * intro_pure; cbn; auto.  *) *)
+  (*   (*     + intro_pure. *) *)
+  (*   (*       go... *) *)
 
-    (*   - destruct o; cbn... *)
-    (*     go... *)
+  (*   (*   - destruct o; cbn... *) *)
+  (*   (*     go... *) *)
 
-    (*   - go. *)
-    (*     rewrite translate_map_monad. *)
-    (*     rewrite interp_cfg3_map_monad. *)
-    (*     apply has_post_bind_strong with (S := ↑ (pure_P g l m)). *)
-    (*     + eapply has_post_weaken. *)
-    (*       apply (map_monad_eutt_state3_ind (fun g' l' m' => pure_P g l m (m',(l',g')))); [| cbn; intuition]. *)
-    (*       * intros * IN (-> & -> & ->). *)
-    (*         destruct a; simpl in *. *)
-    (*         apply has_post_weaken with (↑ (pure_P g l m)). *)
-    (*         apply (H _ IN). *)
-    (*         intro_pure; auto. *)
-    (*       * intro_pure; cbn; auto. *)
-    (*     + intro_pure. *)
-    (*       go... *)
+  (*   (*   - go. *) *)
+  (*   (*     rewrite translate_map_monad. *) *)
+  (*   (*     rewrite interp_cfg3_map_monad. *) *)
+  (*   (*     apply has_post_bind_strong with (S := ↑ (pure_P g l m)). *) *)
+  (*   (*     + eapply has_post_weaken. *) *)
+  (*   (*       apply (map_monad_eutt_state3_ind (fun g' l' m' => pure_P g l m (m',(l',g')))); [| cbn; intuition]. *) *)
+  (*   (*       * intros * IN (-> & -> & ->). *) *)
+  (*   (*         destruct a; simpl in *. *) *)
+  (*   (*         apply has_post_weaken with (↑ (pure_P g l m)). *) *)
+  (*   (*         apply (H _ IN). *) *)
+  (*   (*         intro_pure; auto. *) *)
+  (*   (*       * intro_pure; cbn; auto. *) *)
+  (*   (*     + intro_pure. *) *)
+  (*   (*       go... *) *)
 
-    (*   - destruct o; cbn... *)
-    (*     destruct d; cbn... *)
-    (*     go. *)
-    (*     rewrite translate_map_monad. *)
-    (*     rewrite interp_cfg3_map_monad. *)
-    (*     apply has_post_bind_strong with (S := ↑ (pure_P g l m)). *)
-    (*     + eapply has_post_weaken. *)
-    (*       apply (map_monad_eutt_state3_ind (fun g' l' m' => pure_P g l m (m',(l',g')))); [| cbn; intuition]. *)
-    (*       * intros * IN (-> & -> & ->). *)
-    (*         destruct a; simpl in *. *)
-    (*         apply has_post_weaken with (↑ (pure_P g l m)). *)
-    (*         apply (H _ IN). *)
-    (*         intro_pure; auto. *)
-    (*       * intro_pure; cbn; auto. *)
-    (*     + intro_pure. *)
-    (*       go... *)
+  (*   (*   - destruct o; cbn... *) *)
+  (*   (*     destruct d; cbn... *) *)
+  (*   (*     go. *) *)
+  (*   (*     rewrite translate_map_monad. *) *)
+  (*   (*     rewrite interp_cfg3_map_monad. *) *)
+  (*   (*     apply has_post_bind_strong with (S := ↑ (pure_P g l m)). *) *)
+  (*   (*     + eapply has_post_weaken. *) *)
+  (*   (*       apply (map_monad_eutt_state3_ind (fun g' l' m' => pure_P g l m (m',(l',g')))); [| cbn; intuition]. *) *)
+  (*   (*       * intros * IN (-> & -> & ->). *) *)
+  (*   (*         destruct a; simpl in *. *) *)
+  (*   (*         apply has_post_weaken with (↑ (pure_P g l m)). *) *)
+  (*   (*         apply (H _ IN). *) *)
+  (*   (*         intro_pure; auto. *) *)
+  (*   (*       * intro_pure; cbn; auto. *) *)
+  (*   (*     + intro_pure. *) *)
+  (*   (*       go... *) *)
 
-    (*   - go. *)
-    (*     rewrite translate_map_monad. *)
-    (*     rewrite interp_cfg3_map_monad. *)
-    (*     apply has_post_bind_strong with (S := ↑ (pure_P g l m)). *)
-    (*     + eapply has_post_weaken. *)
-    (*       apply (map_monad_eutt_state3_ind (fun g' l' m' => pure_P g l m (m',(l',g')))); [| cbn; intuition]. *)
-    (*       * intros * IN (-> & -> & ->). *)
-    (*         destruct a; simpl in *. *)
-    (*         apply has_post_weaken with (↑ (pure_P g l m)). *)
-    (*         apply (H _ IN). *)
-    (*         intro_pure; auto. *)
-    (*       * intro_pure; cbn; auto. *)
-    (*     + intro_pure. *)
-    (*       go... *)
+  (*   (*   - go. *) *)
+  (*   (*     rewrite translate_map_monad. *) *)
+  (*   (*     rewrite interp_cfg3_map_monad. *) *)
+  (*   (*     apply has_post_bind_strong with (S := ↑ (pure_P g l m)). *) *)
+  (*   (*     + eapply has_post_weaken. *) *)
+  (*   (*       apply (map_monad_eutt_state3_ind (fun g' l' m' => pure_P g l m (m',(l',g')))); [| cbn; intuition]. *) *)
+  (*   (*       * intros * IN (-> & -> & ->). *) *)
+  (*   (*         destruct a; simpl in *. *) *)
+  (*   (*         apply has_post_weaken with (↑ (pure_P g l m)). *) *)
+  (*   (*         apply (H _ IN). *) *)
+  (*   (*         intro_pure; auto. *) *)
+  (*   (*       * intro_pure; cbn; auto. *) *)
+  (*   (*     + intro_pure. *) *)
+  (*   (*       go... *) *)
 
-    (*   - go. *)
-    (*     rewrite translate_map_monad. *)
-    (*     rewrite interp_cfg3_map_monad. *)
-    (*     apply has_post_bind_strong with (S := ↑ (pure_P g l m)). *)
-    (*     + eapply has_post_weaken. *)
-    (*       apply (map_monad_eutt_state3_ind (fun g' l' m' => pure_P g l m (m',(l',g')))); [| cbn; intuition]. *)
-    (*       * intros * IN (-> & -> & ->). *)
-    (*         destruct a; simpl in *. *)
-    (*         apply has_post_weaken with (↑ (pure_P g l m)). *)
-    (*         apply (H _ IN). *)
-    (*         intro_pure; auto. *)
-    (*       * intro_pure; cbn; auto. *)
-    (*     + intro_pure. *)
-    (*       go... *)
+  (*   (*   - go. *) *)
+  (*   (*     rewrite translate_map_monad. *) *)
+  (*   (*     rewrite interp_cfg3_map_monad. *) *)
+  (*   (*     apply has_post_bind_strong with (S := ↑ (pure_P g l m)). *) *)
+  (*   (*     + eapply has_post_weaken. *) *)
+  (*   (*       apply (map_monad_eutt_state3_ind (fun g' l' m' => pure_P g l m (m',(l',g')))); [| cbn; intuition]. *) *)
+  (*   (*       * intros * IN (-> & -> & ->). *) *)
+  (*   (*         destruct a; simpl in *. *) *)
+  (*   (*         apply has_post_weaken with (↑ (pure_P g l m)). *) *)
+  (*   (*         apply (H _ IN). *) *)
+  (*   (*         intro_pure; auto. *) *)
+  (*   (*       * intro_pure; cbn; auto. *) *)
+  (*   (*     + intro_pure. *) *)
+  (*   (*       go... *) *)
 
-    (*   - go. *)
-    (*     eapply has_post_bind_strong. *)
-    (*     apply (IHe1 (Some t) g l m). *)
-    (*     intros (? & ? & ? & ?) (-> & -> & ->). *)
-    (*     go. *)
-    (*     eapply has_post_bind_strong. *)
-    (*     apply (IHe2 (Some t) g l m). *)
-    (*     intro_pure. *)
-    (*     break_match_goal. *)
-    (*     + go. *)
-    (*       apply has_post_bind_strong with (↑ (pure_P g l m)). *)
-    (*       * unfold concretize_or_pick. *)
-    (*         break_match_goal... *)
-    (*         cbn. *)
-    (*         { *)
-    (*           unfold lift_err. *)
-    (*           break_match_goal... *)
-    (*           go... *)
-    (*         } *)
+  (*   (*   - go. *) *)
+  (*   (*     eapply has_post_bind_strong. *) *)
+  (*   (*     apply (IHe1 (Some t) g l m). *) *)
+  (*   (*     intros (? & ? & ? & ?) (-> & -> & ->). *) *)
+  (*   (*     go. *) *)
+  (*   (*     eapply has_post_bind_strong. *) *)
+  (*   (*     apply (IHe2 (Some t) g l m). *) *)
+  (*   (*     intro_pure. *) *)
+  (*   (*     break_match_goal. *) *)
+  (*   (*     + go. *) *)
+  (*   (*       apply has_post_bind_strong with (↑ (pure_P g l m)). *) *)
+  (*   (*       * unfold concretize_or_pick. *) *)
+  (*   (*         break_match_goal... *) *)
+  (*   (*         cbn. *) *)
+  (*   (*         { *) *)
+  (*   (*           unfold lift_err. *) *)
+  (*   (*           break_match_goal... *) *)
+  (*   (*           go... *) *)
+  (*   (*         } *) *)
 
-    (*       * intro_pure. *)
-    (*         unfold uvalue_to_dvalue_binop2. *)
-    (*         cbn; break_match_goal... *)
-    (*         go... *)
-    (*         break_match_hyp; inv_sum. *)
-    (*         break_match_goal... *)
-    (*         break_match_goal... *)
-    (*         go... *)
+  (*   (*       * intro_pure. *) *)
+  (*   (*         unfold uvalue_to_dvalue_binop2. *) *)
+  (*   (*         cbn; break_match_goal... *) *)
+  (*   (*         go... *) *)
+  (*   (*         break_match_hyp; inv_sum. *) *)
+  (*   (*         break_match_goal... *) *)
+  (*   (*         break_match_goal... *) *)
+  (*   (*         go... *) *)
 
-    (*     + unfold uvalue_to_dvalue_binop. *)
-    (*       cbn. *)
-    (*       break_match_goal. *)
-    (*       go... *)
-    (*       break_match_hyp; try inv_sum. *)
-    (*       break_match_hyp; try inv_sum. *)
-    (*       break_match_goal... *)
-    (*       break_match_goal... *)
-    (*       go... *)
+  (*   (*     + unfold uvalue_to_dvalue_binop. *) *)
+  (*   (*       cbn. *) *)
+  (*   (*       break_match_goal. *) *)
+  (*   (*       go... *) *)
+  (*   (*       break_match_hyp; try inv_sum. *) *)
+  (*   (*       break_match_hyp; try inv_sum. *) *)
+  (*   (*       break_match_goal... *) *)
+  (*   (*       break_match_goal... *) *)
+  (*   (*       go... *) *)
 
-    (*   - go. *)
-    (*     eapply has_post_bind_strong. *)
-    (*     apply (IHe1 (Some t) g l m). *)
-    (*     intro_pure. *)
-    (*     go. *)
-    (*     eapply has_post_bind_strong. *)
-    (*     apply (IHe2 (Some t) g l m). *)
-    (*     intro_pure. *)
-    (*     unfold uvalue_to_dvalue_binop. *)
-    (*     cbn. *)
-    (*     break_match_goal. *)
-    (*     go... *)
-    (*     break_match_hyp; try inv_sum. *)
-    (*     break_match_hyp; try inv_sum. *)
-    (*     break_match_goal... *)
-    (*     break_match_goal... *)
-    (*     go... *)
+  (*   (*   - go. *) *)
+  (*   (*     eapply has_post_bind_strong. *) *)
+  (*   (*     apply (IHe1 (Some t) g l m). *) *)
+  (*   (*     intro_pure. *) *)
+  (*   (*     go. *) *)
+  (*   (*     eapply has_post_bind_strong. *) *)
+  (*   (*     apply (IHe2 (Some t) g l m). *) *)
+  (*   (*     intro_pure. *) *)
+  (*   (*     unfold uvalue_to_dvalue_binop. *) *)
+  (*   (*     cbn. *) *)
+  (*   (*     break_match_goal. *) *)
+  (*   (*     go... *) *)
+  (*   (*     break_match_hyp; try inv_sum. *) *)
+  (*   (*     break_match_hyp; try inv_sum. *) *)
+  (*   (*     break_match_goal... *) *)
+  (*   (*     break_match_goal... *) *)
+  (*   (*     go... *) *)
 
-    (*   - go. *)
-    (*     eapply has_post_bind_strong. *)
-    (*     apply (IHe1 (Some t) g l m). *)
-    (*     intro_pure. *)
-    (*     go. *)
-    (*     eapply has_post_bind_strong. *)
-    (*     apply (IHe2 (Some t) g l m). *)
-    (*     intro_pure. *)
-    (*     break_match_goal. *)
-    (*     + go. *)
-    (*       apply has_post_bind_strong with (↑ (pure_P g l m)). *)
-    (*       * unfold concretize_or_pick. *)
-    (*         break_match_goal... *)
-    (*         cbn. *)
-    (*         { *)
-    (*           unfold lift_err. *)
-    (*           break_match_goal... *)
-    (*           go... *)
-    (*         } *)
+  (*   (*   - go. *) *)
+  (*   (*     eapply has_post_bind_strong. *) *)
+  (*   (*     apply (IHe1 (Some t) g l m). *) *)
+  (*   (*     intro_pure. *) *)
+  (*   (*     go. *) *)
+  (*   (*     eapply has_post_bind_strong. *) *)
+  (*   (*     apply (IHe2 (Some t) g l m). *) *)
+  (*   (*     intro_pure. *) *)
+  (*   (*     break_match_goal. *) *)
+  (*   (*     + go. *) *)
+  (*   (*       apply has_post_bind_strong with (↑ (pure_P g l m)). *) *)
+  (*   (*       * unfold concretize_or_pick. *) *)
+  (*   (*         break_match_goal... *) *)
+  (*   (*         cbn. *) *)
+  (*   (*         { *) *)
+  (*   (*           unfold lift_err. *) *)
+  (*   (*           break_match_goal... *) *)
+  (*   (*           go... *) *)
+  (*   (*         } *) *)
 
-    (*       * intro_pure. *)
-    (*         unfold uvalue_to_dvalue_binop2. *)
-    (*         cbn; break_match_goal. *)
-    (*         go... *)
-    (*         break_match_hyp; inv_sum. *)
-    (*         break_match_goal... *)
-    (*         break_match_goal... *)
-    (*         go... *)
+  (*   (*       * intro_pure. *) *)
+  (*   (*         unfold uvalue_to_dvalue_binop2. *) *)
+  (*   (*         cbn; break_match_goal. *) *)
+  (*   (*         go... *) *)
+  (*   (*         break_match_hyp; inv_sum. *) *)
+  (*   (*         break_match_goal... *) *)
+  (*   (*         break_match_goal... *) *)
+  (*   (*         go... *) *)
 
-    (*     + unfold uvalue_to_dvalue_binop. *)
-    (*       cbn. *)
-    (*       break_match_goal. *)
-    (*       go... *)
-    (*       break_match_hyp; try inv_sum. *)
-    (*       break_match_hyp; try inv_sum. *)
-    (*       break_match_goal... *)
-    (*       break_match_goal... *)
-    (*       go... *)
+  (*   (*     + unfold uvalue_to_dvalue_binop. *) *)
+  (*   (*       cbn. *) *)
+  (*   (*       break_match_goal. *) *)
+  (*   (*       go... *) *)
+  (*   (*       break_match_hyp; try inv_sum. *) *)
+  (*   (*       break_match_hyp; try inv_sum. *) *)
+  (*   (*       break_match_goal... *) *)
+  (*   (*       break_match_goal... *) *)
+  (*   (*       go... *) *)
 
-    (*   - go. *)
-    (*     eapply has_post_bind_strong. *)
-    (*     apply (IHe1 (Some t) g l m). *)
-    (*     intro_pure. *)
-    (*     go. *)
-    (*     eapply has_post_bind_strong. *)
-    (*     apply (IHe2 (Some t) g l m). *)
-    (*     intro_pure. *)
-    (*     unfold uvalue_to_dvalue_binop. *)
-    (*     cbn. *)
-    (*     break_match_goal. *)
-    (*     go... *)
-    (*     break_match_hyp; try inv_sum. *)
-    (*     break_match_hyp; try inv_sum. *)
-    (*     break_match_goal... *)
-    (*     break_match_goal... *)
-    (*     go... *)
+  (*   (*   - go. *) *)
+  (*   (*     eapply has_post_bind_strong. *) *)
+  (*   (*     apply (IHe1 (Some t) g l m). *) *)
+  (*   (*     intro_pure. *) *)
+  (*   (*     go. *) *)
+  (*   (*     eapply has_post_bind_strong. *) *)
+  (*   (*     apply (IHe2 (Some t) g l m). *) *)
+  (*   (*     intro_pure. *) *)
+  (*   (*     unfold uvalue_to_dvalue_binop. *) *)
+  (*   (*     cbn. *) *)
+  (*   (*     break_match_goal. *) *)
+  (*   (*     go... *) *)
+  (*   (*     break_match_hyp; try inv_sum. *) *)
+  (*   (*     break_match_hyp; try inv_sum. *) *)
+  (*   (*     break_match_goal... *) *)
+  (*   (*     break_match_goal... *) *)
+  (*   (*     go... *) *)
 
-    (*   - go. *)
-    (*     eapply has_post_bind_strong. *)
-    (*     apply (IHe (Some t_from) g l m). *)
-    (*     intro_pure. *)
-    (*     unfold uvalue_to_dvalue_uop; cbn. *)
-    (*     break_match_goal. *)
-    (*     go... *)
-    (*     break_match_hyp; try inv_sum. *)
-    (*     unfold ITree.map. *)
-    (*     go. *)
-    (*     apply has_post_bind_strong with (↑ (pure_P g l m)). *)
+  (*   (*   - go. *) *)
+  (*   (*     eapply has_post_bind_strong. *) *)
+  (*   (*     apply (IHe (Some t_from) g l m). *) *)
+  (*   (*     intro_pure. *) *)
+  (*   (*     unfold uvalue_to_dvalue_uop; cbn. *) *)
+  (*   (*     break_match_goal. *) *)
+  (*   (*     go... *) *)
+  (*   (*     break_match_hyp; try inv_sum. *) *)
+  (*   (*     unfold ITree.map. *) *)
+  (*   (*     go. *) *)
+  (*   (*     apply has_post_bind_strong with (↑ (pure_P g l m)). *) *)
 
-    (*     + (* What's the right way to reason about eval_conv? *) *)
-    (*       unfold eval_conv. *)
+  (*   (*     + (* What's the right way to reason about eval_conv? *) *) *)
+  (*   (*       unfold eval_conv. *) *)
 
 
-    (*       pose proof (eval_conv_h_case conv t_from d t_to). *)
-    (*       destruct H as [ (s & H) | [(v & H)| [ (z & H)| (z & H)]] ]. *)
-    (*       rewrite H. *)
+  (*   (*       pose proof (eval_conv_h_case conv t_from d t_to). *) *)
+  (*   (*       destruct H as [ (s & H) | [(v & H)| [ (z & H)| (z & H)]] ]. *) *)
+  (*   (*       rewrite H. *) *)
 
-    (*       destruct t_from; cbn. *)
-    (*       1 - 16 : (rewrite conv_to_exp_raise; rewrite exp_to_instr_raise); trivial_cases. *)
-    (*       destruct d; cbn. *)
-    (*       1 - 14 : (rewrite conv_to_exp_raise; rewrite exp_to_instr_raise); trivial_cases. *)
-    (*       destruct t_from; cbn; rewrite H; go; trivial_cases. *)
+  (*   (*       destruct t_from; cbn. *) *)
+  (*   (*       1 - 16 : (rewrite conv_to_exp_raise; rewrite exp_to_instr_raise); trivial_cases. *) *)
+  (*   (*       destruct d; cbn. *) *)
+  (*   (*       1 - 14 : (rewrite conv_to_exp_raise; rewrite exp_to_instr_raise); trivial_cases. *) *)
+  (*   (*       destruct t_from; cbn; rewrite H; go; trivial_cases. *) *)
 
-    (*       destruct d; cbn; go; trivial_cases. *)
-    (*       rewrite conv_to_exp_raise; rewrite exp_to_instr_raise; trivial_cases. *)
+  (*   (*       destruct d; cbn; go; trivial_cases. *) *)
+  (*   (*       rewrite conv_to_exp_raise; rewrite exp_to_instr_raise; trivial_cases. *) *)
 
-    (*       destruct t_from; rewrite H; try rewrite conv_to_exp_ItoP; try apply ItoP_is_pure. *)
-    (*       destruct d; cbn; go; trivial_cases. *)
+  (*   (*       destruct t_from; rewrite H; try rewrite conv_to_exp_ItoP; try apply ItoP_is_pure. *) *)
+  (*   (*       destruct d; cbn; go; trivial_cases. *) *)
 
-    (*       1 - 13 : apply ItoP_is_pure. *)
+  (*   (*       1 - 13 : apply ItoP_is_pure. *) *)
 
-    (*       rewrite conv_to_exp_raise; rewrite exp_to_instr_raise. apply failure_is_pure. *)
+  (*   (*       rewrite conv_to_exp_raise; rewrite exp_to_instr_raise. apply failure_is_pure. *) *)
 
-    (*       admit. *)
-    (*     + intro_pure. *)
-    (*             go... *)
-    (*   - destruct ptrval; cbn. *)
-    (*     rewrite translate_bind, interp_cfg3_bind. *)
-    (*     eapply has_post_bind_strong. *)
-    (*     apply (IHe (Some d) g l m). *)
-    (*     intro_pure. *)
-    (*     rewrite translate_bind, interp_cfg3_bind. *)
-    (*     rewrite translate_map_monad. *)
-    (*     rewrite interp_cfg3_map_monad. *)
-    (*     apply has_post_bind_strong with (S := ↑ (pure_P g l m)). *)
-    (*     + eapply has_post_weaken. *)
-    (*       apply (map_monad_eutt_state3_ind (fun g' l' m' => pure_P g l m (m',(l',g')))); [| cbn; intuition]. *)
-    (*       * intros * IN (-> & -> & ->). *)
-    (*         destruct a; simpl in *. *)
-    (*         apply has_post_weaken with (↑ (pure_P g l m)). *)
-    (*         apply (H _ IN). *)
-    (*         intro_pure; auto. *)
-    (*       * intro_pure; cbn; auto. *)
-    (*     + intro_pure. *)
-    (*       break_match_goal. *)
-    (*       * rewrite translate_bind, interp_cfg3_bind. *)
-    (*         unfold concretize_or_pick. *)
-    (*         apply has_post_bind_strong with (↑ (pure_P g l m)). *)
-    (*         { *)
-    (*           break_match_goal... *)
-    (*           unfold lift_err. *)
-    (*           break_match_goal... *)
-    (*           cbn; go...  *)
-    (*         } *)
-    (*         intro_pure. *)
-    (*         rewrite translate_bind, interp_cfg3_bind. *)
-    (*         rewrite translate_map_monad. *)
-    (*         rewrite interp_cfg3_map_monad. *)
-    (*         apply has_post_bind_strong with (S := ↑ (pure_P g l m)). *)
-    (*         { eapply has_post_weaken. *)
-    (*           apply (map_monad_eutt_state3_ind (fun g' l' m' => pure_P g l m (m',(l',g')))); [| cbn; intuition]. *)
-    (*           * intros * IN (-> & -> & ->). *)
-    (*             break_match_goal... *)
-    (*             unfold lift_err. *)
-    (*             break_match_goal... *)
-    (*             cbn; go...  *)
-    (*           * intro_pure; cbn; auto. *)
-    (*         } *)
-    (*         intro_pure; cbn; auto. *)
-    (*         unfold ITree.map; go.  *)
-    (*         (* GEP... *) *)
-    (*         unfold interp_cfg3. *)
-    (*         rewrite interp_intrinsics_trigger. *)
-    (*         cbn. *)
-    (*         unfold Intrinsics.F_trigger; cbn. *)
-    (*         rewrite subevent_subevent. *)
-    (*         rewrite interp_global_trigger; cbn. *)
-    (*         rewrite subevent_subevent. *)
-    (*         rewrite interp_local_bind, interp_local_trigger; cbn. *)
-    (*         rewrite subevent_subevent, bind_bind. *)
-    (*         rewrite interp_memory_bind, interp_memory_trigger; cbn. *)
-    (*         rewrite !bind_bind. *)
-    (*         destruct d0; cbn; try (unfold raise; rewrite bind_bind; apply has_post_bind; intros []). *)
-    (*         break_match_goal; cbn; try (unfold raise; rewrite bind_bind; apply has_post_bind; intros []). *)
-    (*         go.  *)
-    (*         rewrite interp_local_ret, interp_memory_ret, bind_ret_l. *)
-    (*         rewrite translate_ret, interp_intrinsics_ret, interp_global_ret, interp_local_ret, interp_memory_ret.  *)
-    (*         go... *)
+  (*   (*       admit. *) *)
+  (*   (*     + intro_pure. *) *)
+  (*   (*             go... *) *)
+  (*   (*   - destruct ptrval; cbn. *) *)
+  (*   (*     rewrite translate_bind, interp_cfg3_bind. *) *)
+  (*   (*     eapply has_post_bind_strong. *) *)
+  (*   (*     apply (IHe (Some d) g l m). *) *)
+  (*   (*     intro_pure. *) *)
+  (*   (*     rewrite translate_bind, interp_cfg3_bind. *) *)
+  (*   (*     rewrite translate_map_monad. *) *)
+  (*   (*     rewrite interp_cfg3_map_monad. *) *)
+  (*   (*     apply has_post_bind_strong with (S := ↑ (pure_P g l m)). *) *)
+  (*   (*     + eapply has_post_weaken. *) *)
+  (*   (*       apply (map_monad_eutt_state3_ind (fun g' l' m' => pure_P g l m (m',(l',g')))); [| cbn; intuition]. *) *)
+  (*   (*       * intros * IN (-> & -> & ->). *) *)
+  (*   (*         destruct a; simpl in *. *) *)
+  (*   (*         apply has_post_weaken with (↑ (pure_P g l m)). *) *)
+  (*   (*         apply (H _ IN). *) *)
+  (*   (*         intro_pure; auto. *) *)
+  (*   (*       * intro_pure; cbn; auto. *) *)
+  (*   (*     + intro_pure. *) *)
+  (*   (*       break_match_goal. *) *)
+  (*   (*       * rewrite translate_bind, interp_cfg3_bind. *) *)
+  (*   (*         unfold concretize_or_pick. *) *)
+  (*   (*         apply has_post_bind_strong with (↑ (pure_P g l m)). *) *)
+  (*   (*         { *) *)
+  (*   (*           break_match_goal... *) *)
+  (*   (*           unfold lift_err. *) *)
+  (*   (*           break_match_goal... *) *)
+  (*   (*           cbn; go...  *) *)
+  (*   (*         } *) *)
+  (*   (*         intro_pure. *) *)
+  (*   (*         rewrite translate_bind, interp_cfg3_bind. *) *)
+  (*   (*         rewrite translate_map_monad. *) *)
+  (*   (*         rewrite interp_cfg3_map_monad. *) *)
+  (*   (*         apply has_post_bind_strong with (S := ↑ (pure_P g l m)). *) *)
+  (*   (*         { eapply has_post_weaken. *) *)
+  (*   (*           apply (map_monad_eutt_state3_ind (fun g' l' m' => pure_P g l m (m',(l',g')))); [| cbn; intuition]. *) *)
+  (*   (*           * intros * IN (-> & -> & ->). *) *)
+  (*   (*             break_match_goal... *) *)
+  (*   (*             unfold lift_err. *) *)
+  (*   (*             break_match_goal... *) *)
+  (*   (*             cbn; go...  *) *)
+  (*   (*           * intro_pure; cbn; auto. *) *)
+  (*   (*         } *) *)
+  (*   (*         intro_pure; cbn; auto. *) *)
+  (*   (*         unfold ITree.map; go.  *) *)
+  (*   (*         (* GEP... *) *) *)
+  (*   (*         unfold interp_cfg3. *) *)
+  (*   (*         rewrite interp_intrinsics_trigger. *) *)
+  (*   (*         cbn. *) *)
+  (*   (*         unfold Intrinsics.F_trigger; cbn. *) *)
+  (*   (*         rewrite subevent_subevent. *) *)
+  (*   (*         rewrite interp_global_trigger; cbn. *) *)
+  (*   (*         rewrite subevent_subevent. *) *)
+  (*   (*         rewrite interp_local_bind, interp_local_trigger; cbn. *) *)
+  (*   (*         rewrite subevent_subevent, bind_bind. *) *)
+  (*   (*         rewrite interp_memory_bind, interp_memory_trigger; cbn. *) *)
+  (*   (*         rewrite !bind_bind. *) *)
+  (*   (*         destruct d0; cbn; try (unfold raise; rewrite bind_bind; apply has_post_bind; intros []). *) *)
+  (*   (*         break_match_goal; cbn; try (unfold raise; rewrite bind_bind; apply has_post_bind; intros []). *) *)
+  (*   (*         go.  *) *)
+  (*   (*         rewrite interp_local_ret, interp_memory_ret, bind_ret_l. *) *)
+  (*   (*         rewrite translate_ret, interp_intrinsics_ret, interp_global_ret, interp_local_ret, interp_memory_ret.  *) *)
+  (*   (*         go... *) *)
 
-    (*       * unfold ITree.map; destruct p; cbn. *)
-    (*         go. *)
-    (*         (* GEP... *) *)
-    (*         unfold interp_cfg3. *)
-    (*         rewrite interp_intrinsics_trigger. *)
-    (*         cbn. *)
-    (*         unfold Intrinsics.F_trigger; cbn. *)
-    (*         rewrite subevent_subevent. *)
-    (*         rewrite interp_global_trigger; cbn. *)
-    (*         rewrite subevent_subevent. *)
-    (*         rewrite interp_local_bind, interp_local_trigger; cbn. *)
-    (*         rewrite subevent_subevent, bind_bind. *)
-    (*         rewrite interp_memory_bind, interp_memory_trigger; cbn. *)
-    (*         rewrite !bind_bind. *)
-    (*         destruct d0; cbn; try (unfold raise; rewrite bind_bind; apply has_post_bind; intros []). *)
-    (*         break_match_goal; cbn; try (unfold raise; rewrite bind_bind; apply has_post_bind; intros []). *)
-    (*         rewrite !bind_ret_l. *)
-    (*         rewrite interp_local_ret, interp_memory_ret, bind_ret_l. *)
-    (*         rewrite translate_ret, interp_intrinsics_ret, interp_global_ret, interp_local_ret, interp_memory_ret.  *)
-    (*         go... *)
+  (*   (*       * unfold ITree.map; destruct p; cbn. *) *)
+  (*   (*         go. *) *)
+  (*   (*         (* GEP... *) *) *)
+  (*   (*         unfold interp_cfg3. *) *)
+  (*   (*         rewrite interp_intrinsics_trigger. *) *)
+  (*   (*         cbn. *) *)
+  (*   (*         unfold Intrinsics.F_trigger; cbn. *) *)
+  (*   (*         rewrite subevent_subevent. *) *)
+  (*   (*         rewrite interp_global_trigger; cbn. *) *)
+  (*   (*         rewrite subevent_subevent. *) *)
+  (*   (*         rewrite interp_local_bind, interp_local_trigger; cbn. *) *)
+  (*   (*         rewrite subevent_subevent, bind_bind. *) *)
+  (*   (*         rewrite interp_memory_bind, interp_memory_trigger; cbn. *) *)
+  (*   (*         rewrite !bind_bind. *) *)
+  (*   (*         destruct d0; cbn; try (unfold raise; rewrite bind_bind; apply has_post_bind; intros []). *) *)
+  (*   (*         break_match_goal; cbn; try (unfold raise; rewrite bind_bind; apply has_post_bind; intros []). *) *)
+  (*   (*         rewrite !bind_ret_l. *) *)
+  (*   (*         rewrite interp_local_ret, interp_memory_ret, bind_ret_l. *) *)
+  (*   (*         rewrite translate_ret, interp_intrinsics_ret, interp_global_ret, interp_local_ret, interp_memory_ret.  *) *)
+  (*   (*         go... *) *)
 
-    (*   - auto... *)
+  (*   (*   - auto... *) *)
 
-    (*   - auto... *)
+  (*   (*   - auto... *) *)
 
-    (*   - auto... *)
+  (*   (*   - auto... *) *)
 
-    (*   - destruct vec; cbn. *)
-    (*     go. *)
-    (*     eapply has_post_bind_strong. *)
-    (*     apply (IHe (Some d) g l m). *)
-    (*     intro_pure. *)
-    (*     clear IHe. *)
-    (*     induction idxs as [| n idxs IH]. *)
-    (*     + cbn. *)
-    (*       go... *)
-    (*     + cbn. *)
-    (*       break_match_goal... *)
-    (*       break_match_goal... *)
-    (*       go... *)
+  (*   (*   - destruct vec; cbn. *) *)
+  (*   (*     go. *) *)
+  (*   (*     eapply has_post_bind_strong. *) *)
+  (*   (*     apply (IHe (Some d) g l m). *) *)
+  (*   (*     intro_pure. *) *)
+  (*   (*     clear IHe. *) *)
+  (*   (*     induction idxs as [| n idxs IH]. *) *)
+  (*   (*     + cbn. *) *)
+  (*   (*       go... *) *)
+  (*   (*     + cbn. *) *)
+  (*   (*       break_match_goal... *) *)
+  (*   (*       break_match_goal... *) *)
+  (*   (*       go... *) *)
     
-    (*   - auto... *)
+  (*   (*   - auto... *) *)
 
-    (*   - destruct cnd,v1,v2; cbn. *)
-    (*     go. *)
-    (*     eapply has_post_bind_strong; [apply IHe | ]. *)
-    (*     intro_pure. *)
-    (*     go. *)
-    (*     eapply has_post_bind_strong; [apply IHe0 |].  *)
-    (*     intro_pure. *)
-    (*     go. *)
-    (*     eapply has_post_bind_strong; [apply IHe1 |].  *)
-    (*     intro_pure. *)
-    (*     break_match_goal. *)
-    (*     go... *)
-    (*     unfold lift_undef_or_err. *)
-    (*     break_match_goal. *)
-    (*     break_match_goal... *)
-    (*     break_match_goal... *)
-    (*     go... *)
+  (*   (*   - destruct cnd,v1,v2; cbn. *) *)
+  (*   (*     go. *) *)
+  (*   (*     eapply has_post_bind_strong; [apply IHe | ]. *) *)
+  (*   (*     intro_pure. *) *)
+  (*   (*     go. *) *)
+  (*   (*     eapply has_post_bind_strong; [apply IHe0 |].  *) *)
+  (*   (*     intro_pure. *) *)
+  (*   (*     go. *) *)
+  (*   (*     eapply has_post_bind_strong; [apply IHe1 |].  *) *)
+  (*   (*     intro_pure. *) *)
+  (*   (*     break_match_goal. *) *)
+  (*   (*     go... *) *)
+  (*   (*     unfold lift_undef_or_err. *) *)
+  (*   (*     break_match_goal. *) *)
+  (*   (*     break_match_goal... *) *)
+  (*   (*     break_match_goal... *) *)
+  (*   (*     go... *) *)
     
-    (*   - destruct v; cbn. *)
-    (*     go. *)
-    (*     eapply has_post_bind_strong. *)
-    (*     apply (IHe (Some d) g l m). *)
-    (*     intro_pure. *)
-    (*     clear IHe. *)
-    (*     go. *)
-    (*     apply has_post_bind_strong with (↑ (pure_P g l m)). *)
-    (*     { unfold pick_your_poison; *)
-    (*         break_match_goal; cbn; *)
-    (*           match goal with *)
-    (*             |- context [Ret _] => rewrite !translate_ret, interp_cfg3_ret; apply eutt_Ret; cbn; auto *)
-    (*           | |- context [concretize_or_pick] => apply concretize_or_pick_is_pure *)
-    (*           | _ => idtac *)
-    (*           end... *)
-    (*     } *)
-    (*     intros (? & ? & ? & ?) (-> & -> & ->). *)
-    (*     go... *)
+  (*   (*   - destruct v; cbn. *) *)
+  (*   (*     go. *) *)
+  (*   (*     eapply has_post_bind_strong. *) *)
+  (*   (*     apply (IHe (Some d) g l m). *) *)
+  (*   (*     intro_pure. *) *)
+  (*   (*     clear IHe. *) *)
+  (*   (*     go. *) *)
+  (*   (*     apply has_post_bind_strong with (↑ (pure_P g l m)). *) *)
+  (*   (*     { unfold pick_your_poison; *) *)
+  (*   (*         break_match_goal; cbn; *) *)
+  (*   (*           match goal with *) *)
+  (*   (*             |- context [Ret _] => rewrite !translate_ret, interp_cfg3_ret; apply eutt_Ret; cbn; auto *) *)
+  (*   (*           | |- context [concretize_or_pick] => apply concretize_or_pick_is_pure *) *)
+  (*   (*           | _ => idtac *) *)
+  (*   (*           end... *) *)
+  (*   (*     } *) *)
+  (*   (*     intros (? & ? & ? & ?) (-> & -> & ->). *) *)
+  (*   (*     go... *) *)
     
-    (* Admitted. *)
+  (*   (* Admitted. *) *)
 
-  End ExpPure.
+  (* End ExpPure. *)
 End ExpLemmas.
